DPE: Finish integrating Pulse hash table into DPE implementation. Wrote not_full utility for pulse hash tables. Can be generalized and put in the hash table library. Wrote utility to free all context structs in a context hash table (not so general).

pulse/share/steel/examples/pulse/dice/dpe/DPE.fst
@@ -12,18 +12,19 @@ module US = FStar.SizeT
 module U8 = FStar.UInt8
 module U32 = FStar.UInt32
 open Array
-open HashTable
 open LinearScanHashTable
 open PulseHashTable
+module PHT = PulseHashTable
+module LSHT = LinearScanHashTable
 open HACL
 open X509
 open EngineTypes
 open L0Types
 open EngineCore
 open L0Core
+open Pulse.Class.BoundedIntegers
 
 friend Pulse.Steel.Wrapper
-#set-options "--print_implicits --print_universes"
 
 (* L1 Context -- to be moved *)
 
@@ -42,7 +43,15 @@ let l1_context_perm (c:l1_context)
     exists_ (fun s -> A.pts_to c.aliasKey_priv full_perm s) `star`
     exists_ (fun s -> A.pts_to c.aliasKey_pub full_perm s) `star`
     exists_ (fun s -> A.pts_to c.aliasKeyCRT full_perm s) `star`
-    exists_ (fun s -> A.pts_to c.deviceIDCSR full_perm s)
+    exists_ (fun s -> A.pts_to c.deviceIDCSR full_perm s) `star`
+    pure (
+      A.is_full_array c.deviceID_priv /\
+      A.is_full_array c.deviceID_pub /\
+      A.is_full_array c.aliasKey_priv /\
+      A.is_full_array c.aliasKey_pub /\
+      A.is_full_array c.aliasKeyCRT /\
+      A.is_full_array c.deviceIDCSR
+    )
 
 let mk_l1_context deviceID_priv deviceID_pub aliasKey_priv aliasKey_pub aliasKeyCRT deviceIDCSR 
   = { deviceID_priv; deviceID_pub; aliasKey_priv; aliasKey_pub; aliasKeyCRT; deviceIDCSR }
@@ -93,6 +102,9 @@ let record_perm (t_rec:record_t) (t_rep:repr_t) : vprop =
 
 (* ----------- GLOBAL STATE ----------- *)
 
+type sid_ref_t = r:R.ref nat & L.lock (exists_ (fun n -> R.pts_to r full_perm n))
+assume val get (#s:pht_sig_us) (ht:ht_t s) (k:s.keyt) : s.valt
+
 assume val dpe_hashf : nat -> US.t
 assume val sht_len : pos_us
 assume val cht_len : pos_us
@@ -111,10 +123,7 @@ fn alloc_ht (#s:pht_sig_us) (l:pos_us)
   let ht = mk_ht l contents;
   let pht = mk_init_pht #s l;
   rewrite (A.pts_to contents full_perm (Seq.create (US.v l) Clean))
-    as (A.pts_to ht.contents full_perm (Seq.create (US.v l) Clean));
-  rewrite (A.pts_to ht.contents full_perm (Seq.create (US.v l) Clean))
     as (A.pts_to ht.contents full_perm pht.repr);
-  assert (pure (US.v ht.sz == pht.sz));
   fold (models s ht pht);
   fold (ht_perm s ht);
   let lk = W.new_lock (ht_perm s ht);
@@ -141,35 +150,144 @@ let sid_ref : sid_ref_t = alloc_sid () ()
 
 (* ----------- IMPLEMENTATION ----------- *)
 
+```pulse
+fn not_full (#s:pht_sig_us) (#pht:erased (pht_t (s_to_ps s))) (ht:ht_t s)
+  requires models s ht pht
+  returns b:bool
+  ensures models s ht pht ** 
+          pure (b ==> LSHT.not_full #(s_to_ps s) #(pht_sz pht) pht.repr)
+{
+  let mut i = 0sz;
+  unfold (models s ht pht);
+
+  while (let vi = !i;  
+    if (vi < ht.sz) { 
+      let c = op_Array_Index ht.contents vi #full_perm #pht.repr; 
+      (Used? c) 
+    } else { false })
+  invariant b. exists (vi:US.t). (
+    A.pts_to ht.contents full_perm pht.repr **
+    R.pts_to i full_perm vi **
+    pure (
+      US.v ht.sz == pht_sz pht /\
+      vi <= ht.sz /\
+      (b == (vi < ht.sz && Used? (pht.repr @@ (US.v vi)))) /\
+      (forall (i:nat). i < US.v vi ==> Used? (pht.repr @@ i))
+    )
+  )
+  {
+    let vi = !i;
+    i := vi + 1sz;
+  };
+  let vi = !i;
+  let res = vi < ht.sz;
+  fold (models s ht pht);
+  res
+}
+```
+
 (*
   OpenSession: Part of DPE API 
   Create a context table and context table lock for the new session. 
   Add the context table lock to the session table. 
   NOTE: Current implementation disregards session protocol 
 *)
-[@@expect_failure]
 ```pulse
 fn open_session (_:unit)
   requires emp
   ensures emp
 {
-  let cht_ref = alloc_ht #cht_sig;
+  let cht = alloc_ht #cht_sig cht_len;
 
-  let sid_lk = dsnd sid_ref;
-  let sht_lk = dsnd locked_sht;
   let sht = dfst locked_sht;
+  let sht_lk = dsnd locked_sht;
+  let sid_lk = dsnd sid_ref;
 
   W.acquire #(exists_ (fun n -> R.pts_to (dfst sid_ref) full_perm n)) sid_lk;
   W.acquire #(ht_perm sht_sig sht) sht_lk;
-  
+
   let sid = !(dfst sid_ref);
 
-  insert sht sid cht_ref;
-  dfst sid_ref := sid + 1;
+  unfold (ht_perm sht_sig sht);
+  with pht. assert (models sht_sig sht pht);
 
-  W.release #(exists_ (fun n -> R.pts_to (dfst sid_ref) full_perm n)) sid_lk;
-  W.release #(ht_perm sht_sig (dfst sht_lk)) sht_lk;
-  ()
+  let b = not_full #sht_sig #pht sht;
+
+  if b {
+    PHT.insert #sht_sig #pht sht sid cht;
+    dfst sid_ref := sid + 1;
+
+    fold (ht_perm sht_sig sht);
+    W.release #(exists_ (fun n -> R.pts_to (dfst sid_ref) full_perm n)) sid_lk;
+    W.release #(ht_perm sht_sig sht) sht_lk;
+  } else {
+    // ERROR -- table full
+    fold (ht_perm sht_sig sht);
+    W.release #(exists_ (fun n -> R.pts_to (dfst sid_ref) full_perm n)) sid_lk;
+    W.release #(ht_perm sht_sig sht) sht_lk;
+  }
+}
+```
+
+```pulse
+fn destroy_cht (ht:ht_t cht_sig)
+  requires ht_perm cht_sig ht
+  ensures emp
+{
+  let mut off = 0sz;
+
+  unfold (ht_perm cht_sig ht);
+  with pht. assert (models cht_sig ht pht);
+  unfold (models cht_sig ht pht);
+
+  while (let voff = !off; (voff < ht.sz))
+  invariant b. exists (voff:US.t). (
+    A.pts_to ht.contents full_perm pht.repr **
+    R.pts_to off full_perm voff **
+    pure (
+      US.v ht.sz == pht.sz /\
+      voff <= ht.sz /\
+      b == (voff < ht.sz)
+    )
+  )
+  {
+    let voff = !off;
+    let c = op_Array_Index ht.contents voff;
+    match c {
+      Used k v -> {
+      let ctxt = dfst v;
+      let ctxt_lk = dsnd v;
+      W.acquire #(context_perm ctxt) ctxt_lk;
+      match ctxt {
+        Engine_context c -> {
+          rewrite (context_perm ctxt) as (engine_context_perm c);
+          unfold (engine_context_perm c);
+          zeroize_array uds_len c.uds #uds_bytes;
+          disable_uds ();
+          free_array c.uds;
+        }
+        L0_context c -> {
+          rewrite (context_perm ctxt) as (l0_context_perm c);
+          unfold (l0_context_perm c);
+          free_array c.cdi;
+        }
+        L1_context c -> {
+          rewrite (context_perm ctxt) as (l1_context_perm c);
+          unfold (l1_context_perm c);
+          free_array c.deviceID_priv;
+          free_array c.deviceID_pub;
+          free_array c.aliasKey_priv;
+          free_array c.aliasKey_pub;
+          free_array c.aliasKeyCRT;
+          free_array c.deviceIDCSR;
+        }
+      }}
+      _ -> {
+        off := voff + 1sz;
+      }
+    }
+  };
+  free_array ht.contents;
 }
 ```
 
@@ -179,27 +297,37 @@ fn open_session (_:unit)
   to it from the session table. 
   NOTE: Current implementation disregards session protocol 
 *)
-[@@expect_failure]
 ```pulse
 fn close_session (sid:nat)
   requires emp
   ensures emp
 {
+  let sht = dfst locked_sht;
   let sht_lk = dsnd locked_sht;
-  W.acquire #(exists_ (fun n -> R.pts_to (dfst locked_sht) full_perm n)) sht_lk;
-  let sht = !(dfst locked_sht);
+  W.acquire #(ht_perm sht_sig sht) sht_lk;
 
-  let cht_ref = get sht sid;
+  unfold (ht_perm sht_sig sht);
+  with pht. assert (models sht_sig sht pht);
 
-  let cht_lk = dsnd cht_ref;
-  W.acquire #(exists_ (fun n -> R.pts_to (dfst cht_ref) full_perm n)) cht_lk;
-  let cht = !(dfst cht_ref);
+  let opt_locked_cht = PHT.lookup #sht_sig #pht sht sid;
 
-  destroy cht;
-  W.release #(exists_ (fun n -> R.pts_to (dfst cht_ref) full_perm n)) cht_lk;
-
-  delete sht sid;
-  W.release #(exists_ (fun n -> R.pts_to (dfst locked_sht) full_perm n)) sht_lk;
+  match opt_locked_cht {
+  Some locked_cht -> { 
+    let cht = dfst locked_cht;
+    let cht_lk = dsnd locked_cht;
+    // Note: We don't release this lock because we give up permission
+    // on the cht when we free its entries by calling destroy_cht
+    W.acquire #(ht_perm cht_sig cht) cht_lk;
+    destroy_cht cht;
+    PHT.delete #sht_sig #pht sht sid;
+    fold (ht_perm sht_sig sht);
+    W.release #(ht_perm sht_sig sht) sht_lk;
+  }
+  None -> {
+    // ERROR -- bad session ID
+    fold (ht_perm sht_sig sht);
+    W.release #(ht_perm sht_sig sht) sht_lk;
+  }}
 }
 ```
 
@@ -222,10 +350,7 @@ fn init_engine_ctxt (uds:A.larray U8.t (US.v uds_len))
 
   rewrite (A.pts_to uds_buf full_perm uds_bytes) 
     as (A.pts_to engine_context.uds full_perm uds_bytes);
-  rewrite (A.pts_to engine_context.uds full_perm uds_bytes `star` 
-           uds_is_enabled `star`
-           pure (A.is_full_array engine_context.uds)) 
-    as (engine_context_perm engine_context);
+  fold (engine_context_perm engine_context);
 
   let ctxt = mk_engine_context_t engine_context;
 
@@ -254,10 +379,7 @@ fn init_l0_ctxt (cdi:A.larray U8.t (US.v dice_digest_len))
   //   as (exists_ (fun s -> A.pts_to l0_context.cdi full_perm s)); 
   drop_ (exists_ (fun (s:elseq U8.t dice_digest_len) -> A.pts_to cdi_buf full_perm s));
   assume_ (exists_ (fun (s:elseq U8.t dice_digest_len) -> A.pts_to l0_context.cdi full_perm s));
-  assume_ (pure(A.is_full_array l0_context.cdi));
-  rewrite (exists_ (fun (s:elseq U8.t dice_digest_len) -> A.pts_to l0_context.cdi full_perm s) 
-          `star` pure (A.is_full_array l0_context.cdi)) 
-    as (l0_context_perm l0_context);
+  fold (l0_context_perm l0_context);
   let ctxt = mk_l0_context_t l0_context;
   rewrite (l0_context_perm l0_context) as (context_perm ctxt);
   let ctxt_lk = W.new_lock (context_perm ctxt);
@@ -303,12 +425,18 @@ fn init_l1_ctxt (deviceIDCSR_len: US.t) (aliasKeyCRT_len: US.t)
   let l1_context = mk_l1_context deviceID_priv_buf deviceID_pub_buf aliasKey_priv_buf aliasKey_pub_buf aliasKeyCRT_buf deviceIDCSR_buf;
 // FIXME: pulse can't prove equality in the following two rewrites 
 // has something to do with not unwrapping the existential
-  // rewrite (exists_ (fun s -> A.pts_to aliasKey_priv full_perm s) `star`
-  //          exists_ (fun s -> A.pts_to aliasKeyCRT full_perm s) `star`
-  //          exists_ (fun s -> A.pts_to deviceIDCSR full_perm s)) 
-  //   as (exists_ (fun s -> A.pts_to l1_context.aliasKey_priv full_perm s) `star`
+  // rewrite (exists_ (fun s -> A.pts_to deviceID_priv_buf full_perm s) `star`
+  //        exists_ (fun s -> A.pts_to deviceID_pub_buf full_perm s) `star`
+  //        exists_ (fun s -> A.pts_to aliasKey_priv_buf full_perm s) `star`
+  //        exists_ (fun s -> A.pts_to aliasKey_pub_buf full_perm s) `star`
+  //        exists_ (fun s -> A.pts_to aliasKeyCRT_buf full_perm s) `star`
+  //        exists_ (fun s -> A.pts_to deviceIDCSR_buf full_perm s))
+  //   as (exists_ (fun s -> A.pts_to l1_context.deviceID_priv full_perm s) `star`
+  //       exists_ (fun s -> A.pts_to l1_context.deviceID_pub full_perm s) `star`
+  //       exists_ (fun s -> A.pts_to l1_context.aliasKey_priv full_perm s) `star`
+  //       exists_ (fun s -> A.pts_to l1_context.aliasKey_pub full_perm s) `star`
   //       exists_ (fun s -> A.pts_to l1_context.aliasKeyCRT full_perm s) `star`
-  //       exists_ (fun s -> A.pts_to l1_context.deviceIDCSR full_perm s)); 
+  //       exists_ (fun s -> A.pts_to l1_context.deviceIDCSR full_perm s));
   drop_ (exists_ (fun s -> A.pts_to deviceID_priv_buf full_perm s) `star`
          exists_ (fun s -> A.pts_to deviceID_pub_buf full_perm s) `star`
          exists_ (fun s -> A.pts_to aliasKey_priv_buf full_perm s) `star`
@@ -321,13 +449,7 @@ fn init_l1_ctxt (deviceIDCSR_len: US.t) (aliasKeyCRT_len: US.t)
            exists_ (fun s -> A.pts_to l1_context.aliasKey_pub full_perm s) `star`
            exists_ (fun s -> A.pts_to l1_context.aliasKeyCRT full_perm s) `star`
            exists_ (fun s -> A.pts_to l1_context.deviceIDCSR full_perm s));
-  rewrite (exists_ (fun s -> A.pts_to l1_context.deviceID_priv full_perm s) `star`
-           exists_ (fun s -> A.pts_to l1_context.deviceID_pub full_perm s) `star`
-           exists_ (fun s -> A.pts_to l1_context.aliasKey_priv full_perm s) `star`
-           exists_ (fun s -> A.pts_to l1_context.aliasKey_pub full_perm s) `star`
-           exists_ (fun s -> A.pts_to l1_context.aliasKeyCRT full_perm s) `star`
-           exists_ (fun s -> A.pts_to l1_context.deviceIDCSR full_perm s)) 
-    as (l1_context_perm l1_context);
+  fold (l1_context_perm l1_context);
   let ctxt = mk_l1_context_t l1_context;
   rewrite (l1_context_perm l1_context) as (context_perm ctxt);
   let ctxt_lk = W.new_lock (context_perm ctxt);
@@ -340,7 +462,6 @@ fn init_l1_ctxt (deviceIDCSR_len: US.t) (aliasKeyCRT_len: US.t)
   Create a context in the initial state (engine context) and store the context
   in the current session's context table. 
 *)
-[@@expect_failure]
 ```pulse
 fn initialize_context (sid:nat) (uds:A.larray U8.t (US.v uds_len))
   requires (
@@ -354,22 +475,49 @@ fn initialize_context (sid:nat) (uds:A.larray U8.t (US.v uds_len))
   let locked_context = init_engine_ctxt uds;
   let ctxt_hndl = prng ();
 
+  let sht = dfst locked_sht;
   let sht_lk = dsnd locked_sht;
-  W.acquire #(exists_ (fun n -> R.pts_to (dfst locked_sht) full_perm n)) sht_lk;
-  let sht = !(dfst locked_sht);
+  W.acquire #(ht_perm sht_sig sht) sht_lk;
 
-  let cht_ref = get sht sid;
+  unfold (ht_perm sht_sig sht);
+  with spht. assert (models sht_sig sht spht);
 
-  let cht_lk = dsnd cht_ref;
-  W.acquire #(exists_ (fun n -> R.pts_to (dfst cht_ref) full_perm n)) cht_lk;
-  let cht = !(dfst cht_ref);
+  let opt_locked_cht = PHT.lookup #sht_sig #spht sht sid;
 
-  store cht ctxt_hndl locked_context;
+  match opt_locked_cht {
+  Some locked_cht -> {
+    let cht = dfst locked_cht;
+    let cht_lk = dsnd locked_cht;
+    W.acquire #(ht_perm cht_sig cht) cht_lk;
 
-  W.release #(exists_ (fun n -> R.pts_to (dfst cht_ref) full_perm n)) cht_lk;
-  W.release #(exists_ (fun n -> R.pts_to (dfst locked_sht) full_perm n)) sht_lk;
-  
-  ctxt_hndl
+    unfold (ht_perm cht_sig cht);
+    with cpht. assert (models cht_sig cht cpht);
+    let b = not_full #cht_sig #cpht cht;
+
+    if b {
+      PHT.insert #cht_sig #cpht cht ctxt_hndl locked_context;
+
+      fold (ht_perm sht_sig sht);
+      fold (ht_perm cht_sig cht);
+      W.release #(ht_perm sht_sig sht) sht_lk;
+      W.release #(ht_perm cht_sig cht) cht_lk;
+      
+      ctxt_hndl
+    } else {
+      // ERROR -- table full
+      fold (ht_perm sht_sig sht);
+      fold (ht_perm cht_sig cht);
+      W.release #(ht_perm sht_sig sht) sht_lk;
+      W.release #(ht_perm cht_sig cht) cht_lk;
+      
+      ctxt_hndl 
+    }}
+  None -> {
+    // ERROR -- bad session ID
+    fold (ht_perm sht_sig sht);
+    W.release #(ht_perm sht_sig sht) sht_lk;
+    0
+  }}
 }
 ```
 
@@ -380,7 +528,6 @@ fn initialize_context (sid:nat) (uds:A.larray U8.t (US.v uds_len))
   and store the new context in the table.
   NOTE: Returns 0 if called when ctxt has type L1_context (bad invocation)
 *)
-[@@expect_failure]
 ```pulse
 fn derive_child (sid:nat) (ctxt_hndl:nat) (record:record_t) (repr:repr_t)
   requires record_perm record repr
@@ -389,171 +536,232 @@ fn derive_child (sid:nat) (ctxt_hndl:nat) (record:record_t) (repr:repr_t)
 {
   let new_ctxt_hndl = prng ();
 
+  let sht = dfst locked_sht;
   let sht_lk = dsnd locked_sht;
-  W.acquire #(exists_ (fun n -> R.pts_to (dfst locked_sht) full_perm n)) sht_lk;
-  let sht = !(dfst locked_sht);
+  W.acquire #(ht_perm sht_sig sht) sht_lk;
 
-  let cht_ref = get sht sid;
+  unfold (ht_perm sht_sig sht);
+  with spht. assert (models sht_sig sht spht);
 
-  let cht_lk = dsnd cht_ref;
-  W.acquire #(exists_ (fun n -> R.pts_to (dfst cht_ref) full_perm n)) cht_lk;
-  let cht = !(dfst cht_ref);
+  let opt_locked_cht = PHT.lookup #sht_sig #spht sht sid;
 
-  let locked_ctxt = get cht ctxt_hndl;
+  match opt_locked_cht {
+  Some locked_cht -> {
+    let cht = dfst locked_cht;
+    let cht_lk = dsnd locked_cht;
+    W.acquire #(ht_perm cht_sig cht) cht_lk;
 
-  let cur_ctxt = dfst locked_ctxt;
-  let ctxt_lk = dsnd locked_ctxt;
-  W.acquire #(context_perm cur_ctxt) ctxt_lk;
+    unfold (ht_perm cht_sig cht);
+    with cpht0. assert (models cht_sig cht cpht0);
 
-  match cur_ctxt {
-  Engine_context ctxt -> {
-    rewrite (context_perm cur_ctxt) as (engine_context_perm ctxt);
-    rewrite (engine_context_perm ctxt) 
-      as (A.pts_to ctxt.uds full_perm uds_bytes `star` 
-          uds_is_enabled `star`
-          pure (A.is_full_array ctxt.uds));
+    let opt_locked_ctxt = PHT.lookup #cht_sig #cpht0 cht ctxt_hndl;
 
-    // NOTE: we won't eventually release engine_context_perm because we won't 
-    // own it anymore -- we will disable the uds and free the uds array
+    match opt_locked_ctxt {
+    Some locked_ctxt -> {
+    let ctxt = dfst locked_ctxt;
+    let ctxt_lk = dsnd locked_ctxt;
+    W.acquire #(context_perm ctxt) ctxt_lk;
 
-    match record {
-    Engine_record r -> {
-      match repr {
-      Engine_repr r0 -> {       
-        rewrite (record_perm record repr) as (engine_record_perm r r0); 
+    match ctxt {
+    Engine_context c -> {
+      // NOTE: we won't eventually release engine_context_perm because we won't 
+      // own it anymore -- we will disable the uds and free the uds array
+      rewrite (context_perm ctxt) as (engine_context_perm c);
+      unfold (engine_context_perm c);
 
-        let cdi = new_array 0uy dice_digest_len;
-        EngineCore.engine_main cdi ctxt.uds r; // FIXME: match on dice return type
-        free_array ctxt.uds;
+      match record {
+      Engine_record r -> {
+        match repr {
+        Engine_repr r0 -> {       
+          rewrite (record_perm record repr) as (engine_record_perm r r0); 
 
-        let new_locked_context = init_l0_ctxt cdi;
-        with s. assert (A.pts_to cdi full_perm s);
-        free_array cdi #(coerce dice_digest_len s);
-        
-        delete cht ctxt_hndl;
-        store cht new_ctxt_hndl new_locked_context;
+          let cdi = new_array 0uy dice_digest_len;
+          EngineCore.engine_main cdi c.uds r; // FIXME: match on dice return type
+          free_array c.uds;
 
-        rewrite (engine_record_perm r r0) as (record_perm record repr);
+          let new_locked_context = init_l0_ctxt cdi;
+          with s. assert (A.pts_to cdi full_perm s);
+          free_array cdi #(coerce dice_digest_len s);
+          
+          PHT.delete #cht_sig #cpht0 cht ctxt_hndl;
+          with cpht1. assert (models cht_sig cht cpht1);
+          let b = not_full #cht_sig #cpht1 cht;
 
-        W.release #(exists_ (fun n -> R.pts_to (dfst cht_ref) full_perm n)) cht_lk;
-        W.release #(exists_ (fun n -> R.pts_to (dfst locked_sht) full_perm n)) sht_lk;
+          if b {
+            PHT.insert #cht_sig #cpht1 cht new_ctxt_hndl new_locked_context; 
 
-        new_ctxt_hndl
+            rewrite (engine_record_perm r r0) as (record_perm record repr);
+
+            fold (ht_perm sht_sig sht);
+            fold (ht_perm cht_sig cht);
+            W.release #(ht_perm sht_sig sht) sht_lk;
+            W.release #(ht_perm cht_sig cht) cht_lk;
+
+            new_ctxt_hndl
+          } else {
+            // ERROR -- table full
+            rewrite (engine_record_perm r r0) as (record_perm record repr);
+
+            fold (ht_perm sht_sig sht);
+            fold (ht_perm cht_sig cht);
+            W.release #(ht_perm sht_sig sht) sht_lk;
+            W.release #(ht_perm cht_sig cht) cht_lk;
+
+            new_ctxt_hndl
+          }
+        }
+        _ -> {
+          // ERROR - repr should have type (Egnine_repr r0)
+          zeroize_array uds_len c.uds #uds_bytes;
+          disable_uds ();
+          free_array c.uds;
+
+          fold (ht_perm sht_sig sht);
+          fold (ht_perm cht_sig cht);
+          W.release #(ht_perm sht_sig sht) sht_lk;
+          W.release #(ht_perm cht_sig cht) cht_lk;
+          0
+        }}
       }
       _ -> {
-        // ERROR - bad invocation of DeriveChild
-        zeroize_array uds_len ctxt.uds #uds_bytes;
+        // ERROR - record should have type (Engine_record r)
+        zeroize_array uds_len c.uds;
         disable_uds ();
-        free_array ctxt.uds;
+        free_array c.uds;
 
-        W.release #(exists_ (fun n -> R.pts_to (dfst cht_ref) full_perm n)) cht_lk;
-        W.release #(exists_ (fun n -> R.pts_to (dfst locked_sht) full_perm n)) sht_lk;
+        fold (ht_perm sht_sig sht);
+        fold (ht_perm cht_sig cht);
+        W.release #(ht_perm sht_sig sht) sht_lk;
+        W.release #(ht_perm cht_sig cht) cht_lk;
         0
       }}
     }
-    _ -> {
-      // ERROR - bad invocation of DeriveChild
-      zeroize_array uds_len ctxt.uds;
-      disable_uds ();
-      free_array ctxt.uds;
+    L0_context c -> {    
+      // NOTE: we won't eventually release l0_context_perm because we won't 
+      // own it anymore -- we will free the cdi array
+      rewrite (context_perm ctxt) as (l0_context_perm c);
+      unfold (l0_context_perm c);
 
-      W.release #(exists_ (fun n -> R.pts_to (dfst cht_ref) full_perm n)) cht_lk;
-      W.release #(exists_ (fun n -> R.pts_to (dfst locked_sht) full_perm n)) sht_lk;
-      0
-    }}
-  }
-  L0_context ctxt -> {
-    rewrite (context_perm cur_ctxt) as (l0_context_perm ctxt);
-    rewrite (l0_context_perm ctxt) 
-      as (exists_ (fun (s:elseq U8.t dice_digest_len) -> A.pts_to ctxt.cdi full_perm s) `star`
-          pure (A.is_full_array ctxt.cdi));
+      with s. assert (A.pts_to c.cdi full_perm s);
 
-    with s. assert (A.pts_to ctxt.cdi full_perm s);
+      match record {
+      L0_record r -> {
+        match repr {
+        L0_repr r0 -> {
+          let idcsr_ing = r.deviceIDCSR_ingredients;
+          let akcrt_ing = r.aliasKeyCRT_ingredients;
 
-    // NOTE: we won't eventually release l0_context_perm because we won't 
-    // own it anymore -- we will free the cdi array
+          let deviceIDCRI_len = len_of_deviceIDCRI  idcsr_ing.version idcsr_ing.s_common 
+                                                    idcsr_ing.s_org idcsr_ing.s_country;
+          let aliasKeyTBS_len = len_of_aliasKeyTBS  akcrt_ing.serialNumber akcrt_ing.i_common 
+                                                    akcrt_ing.i_org akcrt_ing.i_country 
+                                                    akcrt_ing.s_common akcrt_ing.s_org 
+                                                    akcrt_ing.s_country akcrt_ing.l0_version;
+          let deviceIDCSR_len = length_of_deviceIDCSR deviceIDCRI_len;
+          let aliasKeyCRT_len = length_of_aliasKeyCRT aliasKeyTBS_len;
 
-    match record {
-    L0_record r -> {
-      match repr {
-      L0_repr r0 -> {
-        let idcsr_ing = r.deviceIDCSR_ingredients;
-        let akcrt_ing = r.aliasKeyCRT_ingredients;
+          let deviceID_pub = new_array 0uy v32us;
+          let deviceID_priv = new_array 0uy v32us;
+          let aliasKey_pub = new_array 0uy v32us;
+          let aliasKey_priv = new_array 0uy v32us;
+          let deviceIDCSR = new_array 0uy deviceIDCSR_len;
+          let aliasKeyCRT = new_array 0uy aliasKeyCRT_len;
 
-        let deviceIDCRI_len = len_of_deviceIDCRI  idcsr_ing.version idcsr_ing.s_common 
-                                                  idcsr_ing.s_org idcsr_ing.s_country;
-        let aliasKeyTBS_len = len_of_aliasKeyTBS  akcrt_ing.serialNumber akcrt_ing.i_common 
-                                                  akcrt_ing.i_org akcrt_ing.i_country 
-                                                  akcrt_ing.s_common akcrt_ing.s_org 
-                                                  akcrt_ing.s_country akcrt_ing.l0_version;
-        let deviceIDCSR_len = length_of_deviceIDCSR deviceIDCRI_len;
-        let aliasKeyCRT_len = length_of_aliasKeyCRT aliasKeyTBS_len;
+          rewrite (record_perm record repr) as (l0_record_perm r r0); 
 
-        let deviceID_pub = new_array 0uy v32us;
-        let deviceID_priv = new_array 0uy v32us;
-        let aliasKey_pub = new_array 0uy v32us;
-        let aliasKey_priv = new_array 0uy v32us;
-        let deviceIDCSR = new_array 0uy deviceIDCSR_len;
-        let aliasKeyCRT = new_array 0uy aliasKeyCRT_len;
+          assume_ (pure(valid_hkdf_ikm_len (digest_len dice_hash_alg)));
+          
+          L0Core.l0_main  c.cdi deviceID_pub deviceID_priv 
+                          aliasKey_pub aliasKey_priv 
+                          aliasKeyTBS_len aliasKeyCRT_len aliasKeyCRT 
+                          deviceIDCRI_len deviceIDCSR_len deviceIDCSR r;
+          free_array c.cdi;
 
-        rewrite (record_perm record repr) as (l0_record_perm r r0); 
+          with (s1:elseq U8.t v32us). assert (A.pts_to aliasKey_priv full_perm s1);
+          let new_locked_context = init_l1_ctxt deviceIDCSR_len aliasKeyCRT_len 
+                                                deviceID_priv deviceID_pub
+                                                aliasKey_priv aliasKey_pub 
+                                                deviceIDCSR aliasKeyCRT;
+          free_array deviceID_pub;
+          free_array deviceID_priv;
+          free_array aliasKey_pub;
+          free_array aliasKey_priv;
+          free_array deviceIDCSR;
+          free_array aliasKeyCRT;
+          
+          PHT.delete #cht_sig #cpht0 cht ctxt_hndl;
+          with cpht1. assert (models cht_sig cht cpht1);
+          let b = not_full #cht_sig #cpht1 cht;
 
-        assume_ (pure(valid_hkdf_ikm_len (digest_len dice_hash_alg)));
-        
-        L0Core.l0_main  ctxt.cdi deviceID_pub deviceID_priv 
-                        aliasKey_pub aliasKey_priv 
-                        aliasKeyTBS_len aliasKeyCRT_len aliasKeyCRT 
-                        deviceIDCRI_len deviceIDCSR_len deviceIDCSR r;
-        free_array ctxt.cdi;
+          if b {
+            PHT.insert #cht_sig #cpht1 cht new_ctxt_hndl new_locked_context;
 
-        with (s1:elseq U8.t v32us). assert (A.pts_to aliasKey_priv full_perm s1);
-        let new_locked_context = init_l1_ctxt deviceIDCSR_len aliasKeyCRT_len 
-                                              deviceID_priv deviceID_pub
-                                              aliasKey_priv aliasKey_pub 
-                                              deviceIDCSR aliasKeyCRT;
-        free_array deviceID_pub;
-        free_array deviceID_priv;
-        free_array aliasKey_pub;
-        free_array aliasKey_priv;
-        free_array deviceIDCSR;
-        free_array aliasKeyCRT;
-        
-        delete cht ctxt_hndl;
-        store cht new_ctxt_hndl new_locked_context;
+            rewrite (l0_record_perm r r0) as (record_perm record repr);
 
-        rewrite (l0_record_perm r r0) as (record_perm record repr);
+            fold (ht_perm sht_sig sht);
+            fold (ht_perm cht_sig cht);
+            W.release #(ht_perm sht_sig sht) sht_lk;
+            W.release #(ht_perm cht_sig cht) cht_lk;
 
-        W.release #(exists_ (fun n -> R.pts_to (dfst cht_ref) full_perm n)) cht_lk;
-        W.release #(exists_ (fun n -> R.pts_to (dfst locked_sht) full_perm n)) sht_lk;
+            new_ctxt_hndl
+          } else {
+            // ERROR -- table full
+            rewrite (l0_record_perm r r0) as (record_perm record repr);
 
-        new_ctxt_hndl
+            fold (ht_perm sht_sig sht);
+            fold (ht_perm cht_sig cht);
+            W.release #(ht_perm sht_sig sht) sht_lk;
+            W.release #(ht_perm cht_sig cht) cht_lk;
+
+            new_ctxt_hndl
+          }
+        }
+        _ -> {
+          // ERROR - repr should have type (L0_repr r0)
+          zeroize_array dice_digest_len c.cdi;
+          free_array c.cdi;
+
+          fold (ht_perm sht_sig sht);
+          fold (ht_perm cht_sig cht);
+          W.release #(ht_perm sht_sig sht) sht_lk;
+          W.release #(ht_perm cht_sig cht) cht_lk;
+          0
+        }}
       }
       _ -> {
-        // ERROR - bad invocation of DeriveChild
-        zeroize_array dice_digest_len ctxt.cdi;
-        free_array ctxt.cdi;
+        // ERROR - record should have type (L0_record r)
+        zeroize_array dice_digest_len c.cdi;
+        free_array c.cdi;
 
-        W.release #(exists_ (fun n -> R.pts_to (dfst cht_ref) full_perm n)) cht_lk;
-        W.release #(exists_ (fun n -> R.pts_to (dfst locked_sht) full_perm n)) sht_lk;
+        fold (ht_perm sht_sig sht);
+        fold (ht_perm cht_sig cht);
+        W.release #(ht_perm sht_sig sht) sht_lk;
+        W.release #(ht_perm cht_sig cht) cht_lk;
         0
       }}
     }
-    _ -> {
+    _ -> { 
       // ERROR - bad invocation of DeriveChild
-      zeroize_array dice_digest_len ctxt.cdi;
-      free_array ctxt.cdi;
-
-      W.release #(exists_ (fun n -> R.pts_to (dfst cht_ref) full_perm n)) cht_lk;
-      W.release #(exists_ (fun n -> R.pts_to (dfst locked_sht) full_perm n)) sht_lk;
+      fold (ht_perm sht_sig sht);
+      fold (ht_perm cht_sig cht);
+      W.release #(context_perm ctxt) ctxt_lk;
+      W.release #(ht_perm sht_sig sht) sht_lk;
+      W.release #(ht_perm cht_sig cht) cht_lk;
       0
-    }}
-  }
-  _ -> { 
-    // ERROR - bad invocation of DeriveChild
-    W.release #(context_perm cur_ctxt) ctxt_lk;
-    W.release #(exists_ (fun n -> R.pts_to (dfst cht_ref) full_perm n)) cht_lk;
-    W.release #(exists_ (fun n -> R.pts_to (dfst locked_sht) full_perm n)) sht_lk;
+    }}}
+    None -> { 
+    // ERROR -- cannot invoke DeriveChild with L1 context
+    fold (ht_perm sht_sig sht);
+    fold (ht_perm cht_sig cht);
+    W.release #(ht_perm sht_sig sht) sht_lk;
+    W.release #(ht_perm cht_sig cht) cht_lk;
     0
+    }}}
+  None -> { 
+  // ERROR - bad session ID
+  fold (ht_perm sht_sig sht);
+  W.release #(ht_perm sht_sig sht) sht_lk;
+  0
   }}
 }
 ```
